updates

generic/Zeta.AppSimulate.fsti
@@ -64,18 +64,34 @@ let simulate_step #aprm (fncall: appfn_call aprm) (st: app_state aprm.adm):
 (* the result of a function. We need this type since the we cannot simply define a
  * seq (result), since the result type depends on the function id.
  *)
-type appfn_call_res (aprm: app_params) =
-  | FnRes: fid_res: appfn_id aprm -> res: appfn_res fid_res -> appfn_call_res aprm
+type appfn_call_res (aprm: app_params) = {
+  fid_res: appfn_id aprm;
+  res: appfn_res fid_res;
+}
+(*  | FnRes: fid_res: appfn_id aprm -> res: appfn_res fid_res -> appfn_call_res aprm *)
 
 (* initial state of the application *)
 let init_app_state (adm: app_data_model): app_state adm =
   fun _ -> Null
 
+(* a call sequence and a result sequence are consistent if they have the same function id at the
+ * same positions of each sequence
+ *)
 let consistent #aprm (call_seq: S.seq (appfn_call aprm)) (res_seq: S.seq (appfn_call_res aprm)) =
   S.length call_seq = S.length res_seq /\
   (forall (i: SA.seq_index call_seq).
     {:pattern ((S.index call_seq i).fid_call = (S.index res_seq i).fid_res)}
     (S.index call_seq i).fid_call = (S.index res_seq i).fid_res)
+
+(* if we have a consistent call and result sequence we can extend each with a new entry having
+ * the same fid and the result sequences will be consistent *)
+val consistent_extend (#aprm: app_params)
+  (call_seq: S.seq (appfn_call aprm))
+  (res_seq: S.seq (appfn_call_res aprm){consistent call_seq res_seq})
+  (c: appfn_call aprm)
+  (r: appfn_call_res aprm)
+  : Lemma (requires (c.fid_call = r.fid_res))
+          (ensures (consistent (SA.append1 call_seq c) (SA.append1 res_seq r)))
 
 let rec simulate #aprm (fs: S.seq (appfn_call aprm)):
   Tot (or: option (app_state aprm.adm & S.seq (appfn_call_res aprm))
@@ -83,5 +99,22 @@ let rec simulate #aprm (fs: S.seq (appfn_call aprm)):
                        consistent fs rs)})
   (decreases (S.length fs)) =
   let n = S.length fs in
-
-  admit()
+  if n = 0 then
+    Some (init_app_state aprm.adm, S.empty #(appfn_call_res aprm))
+  else
+    let fs' = SA.prefix fs (n-1) in
+    let ors = simulate fs' in
+    if None? ors then None
+    else
+      let Some (st', rs') = ors in
+      let c = S.index fs (n-1) in
+      let or = simulate_step c st' in
+      if None? or then None
+      else (
+        let Some (st, r) = or in
+        let r = {fid_res = c.fid_call; res = r} in
+        let rs = SA.append1 rs' r in
+        consistent_extend fs' rs' c r;
+        SA.lemma_hprefix_append_telem fs;
+        Some (st, rs)
+      )
